defined message, message slice and server

src/program_proof/session/definitions.v
@@ -86,8 +86,8 @@ Section heap.
              IntoVal_def := (IntoVal_def Slice.t, W64 0);
            |}.
     destruct v as [[a []] d]; done. 
-  Defined. 
-
+  Defined.
+  
   #[global] Instance operation_into_val_for_type : IntoValForType (Slice.t*u64) (struct.t Operation).
   Proof. constructor; auto. Qed.
 
@@ -99,13 +99,10 @@ Section heap.
   Definition operation_slice' (op_s: Slice.t) (op: list Operation.t)
                               (n: nat) : iProp Σ :=
     ∃ ops , own_slice op_s (struct.t Operation) (DfracOwn 1) (ops) ∗
-            [∗ list] _ ↦ opv;o ∈ ops;op , (is_operation opv o n).
+            [∗ list] _ ↦ opv;o ∈ ops;op, is_operation opv o n.
   
-  Definition operation_slice (s: Slice.t) (ls: list Operation.t) (n: nat) : iProp Σ :=
-    operation_slice' s ls n.
-
-  Definition operation_to_val (o: Operation.t) (s: Slice.t) :=
-    (s, (#o.(Operation.Data), #()))%V.
+  Definition operation_slice (s: Slice.t) (l: list Operation.t) (n: nat) : iProp Σ :=
+    operation_slice' s l n.
 
   Definition message_val (msg:u64*u64*u64*u64*u64*Slice.t*u64*u64*Slice.t*u64*u64*u64*u64*u64*u64*Slice.t*u64*u64) : val :=
     (#msg.1.1.1.1.1.1.1.1.1.1.1.1.1.1.1.1.1,
@@ -134,6 +131,69 @@ Section heap.
 
   Hint Resolve message_val_t : core.
   
+  Definition message_from_val (v : val) :=
+    match v with
+    | (#(LitInt MessageType),
+         (#(LitInt C2S_Client_Id),
+            (#(LitInt C2S_Server_Id),
+               (#(LitInt C2S_Client_OperationType),
+                  (#(LitInt C2S_Client_Data),
+                     (C2S_Client_VersionVector,
+                        (#(LitInt S2S_Gossip_Sending_ServerId),
+                           (#(LitInt S2S_Gossip_Receiving_ServerId),
+                              (S2S_Gossip_Operations,
+                                 (#(LitInt S2S_Gossip_Index),
+                                    (#(LitInt S2S_Acknowledge_Gossip_Sending_ServerId),
+                                       (#(LitInt S2S_Acknowledge_Gossip_Receiving_ServerId),
+                                          (#(LitInt S2S_Acknowledge_Gossip_Index),
+                                             (#(LitInt S2C_Client_OperationType),
+                                                (#(LitInt S2C_Client_Data),
+                                                   (S2C_Client_VersionVector,
+                                                      (#(LitInt S2C_Server_Id),
+                                                         (#(LitInt S2C_Client_Number), #()))))))))))))))))))%V =>
+        match ((from_val C2S_Client_VersionVector: option Slice.t),
+                 (from_val S2S_Gossip_Operations: option Slice.t),
+                   (from_val S2C_Client_VersionVector: option Slice.t)) with
+        | (Some s1, Some s2, Some s3) => Some (MessageType,
+                                                 C2S_Client_Id,
+                                                   C2S_Server_Id,
+                                                     C2S_Client_OperationType,
+                                                       C2S_Client_Data,
+                                                         s1, 
+                                                           S2S_Gossip_Sending_ServerId,
+                                                             S2S_Gossip_Receiving_ServerId, s2, S2S_Gossip_Index,
+                                                               S2S_Acknowledge_Gossip_Sending_ServerId,
+                                                                 S2S_Acknowledge_Gossip_Receiving_ServerId,
+                                                                   S2S_Acknowledge_Gossip_Index,
+                                                                     S2C_Client_OperationType,
+                                                                       S2C_Client_Data,
+                                                                         s3,
+                                                                           S2C_Server_Id,
+                                                                             S2C_Client_Number)
+        | _ => None
+        end
+    | _ => None
+  end.
+  
+  Global Instance message_into_val : IntoVal (u64*u64*u64*u64*u64*Slice.t*u64*u64*Slice.t*u64*u64*u64*u64*u64*u64*Slice.t*u64*u64).
+  Proof.
+    refine {| into_val.to_val := message_val;
+             from_val := message_from_val ;
+             IntoVal_def := (W64 0, W64 0, W64 0, W64 0, W64 0,
+                               IntoVal_def Slice.t, W64 0, W64 0,
+                                 IntoVal_def Slice.t,
+                                   W64 0, W64 0, W64 0, W64 0, W64 0,
+                                     W64 0, IntoVal_def Slice.t,
+                                       W64 0, W64 0);
+           |}.
+    destruct v. repeat destruct p. simpl. f_equal.
+    destruct t1. destruct t0. destruct t.
+    simpl. auto.
+  Defined. 
+
+  #[global] Instance message_into_val_for_type : IntoValForType (u64*u64*u64*u64*u64*Slice.t*u64*u64*Slice.t*u64*u64*u64*u64*u64*u64*Slice.t*u64*u64) (struct.t server.Message).
+  Proof. constructor; auto. simpl. repeat split; auto. Qed.
+  
   Definition is_message (msgv: u64*u64*u64*u64*u64*Slice.t*u64*u64*Slice.t*u64*u64*u64*u64*u64*u64*Slice.t*u64*u64)
     (msg: Message.t) (msgv_len: nat): iProp Σ :=
     ⌜msgv.1.1.1.1.1.1.1.1.1.1.1.1.1.1.1.1.1 = msg.(Message.MessageType)⌝ ∗
@@ -156,5 +216,25 @@ Section heap.
     own_slice_small msgv.1.1.2 uint64T DfracDiscarded msg.(Message.S2C_Client_VersionVector) ∗
     ⌜msgv.1.2 = msg.(Message.S2C_Server_Id)⌝ ∗
     ⌜msgv.2 = msg.(Message.S2C_Client_Number)⌝.
+
+  Definition message_slice' (msg_s: Slice.t) (msg: list Message.t)
+                              (n: nat) : iProp Σ :=
+    ∃ msgs, own_slice msg_s (struct.t server.Message) (DfracOwn 1) msgs ∗
+            [∗ list] _ ↦ mv;m ∈ msgs;msg, is_message mv m n.
+  
+  Definition message_slice (s: Slice.t) (l: list Message.t) (n: nat) : iProp Σ :=
+    message_slice' s l n.
+
+  Definition is_server (sv: u64*u64*Slice.t*Slice.t*Slice.t*Slice.t*Slice.t*Slice.t) (s: Server.t) (sv_len: nat): iProp Σ :=
+    ⌜sv.1.1.1.1.1.1.1 = s.(Server.Id)⌝ ∗
+    ⌜sv.1.1.1.1.1.1.2 = s.(Server.NumberOfServers)⌝ ∗
+    message_slice sv.1.1.1.1.1.2 s.(Server.UnsatisfiedRequests) sv_len ∗
+    ⌜sv_len = length s.(Server.UnsatisfiedRequests)⌝ ∗
+    own_slice_small sv.1.1.1.1.2 uint64T DfracDiscarded s.(Server.VectorClock) ∗
+    operation_slice sv.1.1.1.2 s.(Server.OperationsPerformed) sv_len ∗
+    operation_slice sv.1.1.2 s.(Server.MyOperations) sv_len ∗
+    operation_slice sv.1.2 s.(Server.PendingOperations) sv_len ∗
+    ⌜sv_len = length s.(Server.GossipAcknowledgements)⌝ ∗
+    own_slice_small sv.2 uint64T DfracDiscarded s.(Server.GossipAcknowledgements).
 
 End heap.
